Tried to replace reveal by showing the property with pkenc_input but failed

src/lib/communication/DY.Lib.Communication.Core.fst
@@ -21,9 +21,33 @@ type communication_message = {
 %splice [ps_communication_message_is_well_formed] (gen_is_well_formed_lemma (`communication_message))
 
 [@@with_bytes bytes]
+type pkenc_input =
+  | PkEncInput: payload:bytes -> pkenc_input
+  | PkEncSignInput: cm:communication_message -> pkenc_input
+
+#push-options "--ifuel 1 --fuel 0"
+%splice [ps_pkenc_input] (gen_parser (`pkenc_input))
+%splice [ps_pkenc_input_is_well_formed] (gen_is_well_formed_lemma (`pkenc_input))
+#pop-options
+
+instance parseable_serializeable_bytes_pkenc_input: parseable_serializeable bytes pkenc_input
+  = mk_parseable_serializeable ps_pkenc_input
+
+[@@with_bytes bytes]
+type signature_input = 
+  | Plain: msg:communication_message -> signature_input
+  | Encrypted: payload:bytes -> signature_input
+
+#push-options "--ifuel 1 --fuel 0"
+%splice [ps_signature_input] (gen_parser (`signature_input))
+%splice [ps_signature_input_is_well_formed] (gen_is_well_formed_lemma (`signature_input))
+#pop-options
+
+instance parseable_serializeable_bytes_signature_input: parseable_serializeable bytes signature_input
+  = mk_parseable_serializeable ps_signature_input
+
+[@@with_bytes bytes]
 type communication_message_sign = {
-  sender:principal;
-  receiver:principal;
   payload:bytes;
   signature:bytes;
 }
@@ -34,18 +58,6 @@ type communication_message_sign = {
 instance parseable_serializeable_bytes_communication_message_sign: parseable_serializeable bytes communication_message_sign
   = mk_parseable_serializeable ps_communication_message_sign
 
-[@@with_bytes bytes]
-type signature_input = 
-  | Plain: msg:communication_message -> signature_input
-  | Encrypted: msg:communication_message -> signature_input
-
-#push-options "--ifuel 1 --fuel 0"
-%splice [ps_signature_input] (gen_parser (`signature_input))
-%splice [ps_signature_input_is_well_formed] (gen_is_well_formed_lemma (`signature_input))
-#pop-options
-
-instance parseable_serializeable_bytes_signature_input: parseable_serializeable bytes signature_input
-  = mk_parseable_serializeable ps_signature_input
 
 (*** Events ***)
 
@@ -91,9 +103,10 @@ let comm_label sender receiver = join (principal_label sender) (principal_label 
 
 (**** Confidential Send and Receive Functions ****)
 
-val encrypt_message: bytes -> bytes -> bytes -> bytes
+val encrypt_message: bytes -> bytes -> pkenc_input -> bytes
 let encrypt_message pk_receiver nonce payload =
-  pk_enc pk_receiver nonce payload
+  let payload_bytes = serialize pkenc_input payload in
+  pk_enc pk_receiver nonce payload_bytes
 
 val send_confidential:
   communication_keys_sess_ids ->
@@ -103,14 +116,15 @@ let send_confidential comm_keys_ids sender receiver payload =
   let*? pk_receiver = get_public_key sender comm_keys_ids.pki (LongTermPkEncKey comm_layer_pkenc_tag) receiver in
   let* nonce = mk_rand PkNonce (long_term_key_label sender) 32 in
   trigger_event sender (CommConfSendMsg sender receiver payload);*
-  let msg_encrypted = encrypt_message pk_receiver nonce payload in
+  let msg_encrypted = encrypt_message pk_receiver nonce (PkEncInput payload) in
   let* msg_id = send_msg msg_encrypted in  
   return (Some msg_id)
 
 
-val decrypt_message: bytes -> bytes -> option bytes
+val decrypt_message: bytes -> bytes -> option pkenc_input
 let decrypt_message sk_receiver msg_encrypted =
-  pk_dec sk_receiver msg_encrypted
+  let? payload_bytes = pk_dec sk_receiver msg_encrypted in
+  parse pkenc_input payload_bytes
 
 val receive_confidential:
   communication_keys_sess_ids ->
@@ -119,7 +133,9 @@ val receive_confidential:
 let receive_confidential comm_keys_ids receiver msg_id =
   let*? sk_receiver = get_private_key receiver comm_keys_ids.private_keys (LongTermPkEncKey comm_layer_pkenc_tag) in
   let*? msg_encrypted = recv_msg msg_id in
-  let*? payload = return (decrypt_message sk_receiver msg_encrypted) in
+  let*? pkenc_in:pkenc_input = return (decrypt_message sk_receiver msg_encrypted) in
+  return (guard (PkEncInput? pkenc_in));*?
+  let payload = PkEncInput?.payload pkenc_in in
   trigger_event receiver (CommConfReceiveMsg receiver payload);*
   return (Some payload)
 
@@ -129,16 +145,16 @@ let receive_confidential comm_keys_ids receiver msg_id =
 val sign_message: principal -> principal -> bytes -> bool -> bytes -> bytes -> bytes
 let sign_message sender receiver payload is_encrypted sk nonce =
   if is_encrypted then (
-    let sig_input = Encrypted {sender; receiver; payload} in
+    let sig_input = Encrypted payload in
     let sig_input_bytes = serialize signature_input sig_input in
     let signature = sign sk nonce sig_input_bytes in
-    let msg_signed = {sender; receiver; payload; signature} in
+    let msg_signed = {payload=sig_input_bytes; signature} in
     serialize communication_message_sign msg_signed
   ) else (
     let sig_input = Plain {sender; receiver; payload} in
     let sig_input_bytes = serialize signature_input sig_input in
     let signature = sign sk nonce sig_input_bytes in
-    let msg_signed = {sender; receiver; payload; signature} in
+    let msg_signed = {payload=sig_input_bytes; signature} in
     serialize communication_message_sign msg_signed
   )
 
@@ -154,49 +170,53 @@ let send_authenticated comm_keys_ids sender receiver payload =
   let* msg_id = send_msg msg_signed in
   return (Some msg_id)
 
-
-val verify_message: principal -> bytes -> bool -> bytes -> option communication_message
+#push-options "--ifuel 1 --fuel 0"
+val verify_message: principal -> bytes -> bool -> bytes -> option bytes
 let verify_message receiver msg_bytes is_encrypted vk_sender =
   let? msg_signed = parse communication_message_sign msg_bytes in
-  if is_encrypted then (
-    let sig_input = Encrypted {sender=msg_signed.sender; receiver=msg_signed.receiver; payload=msg_signed.payload} in
-    let sig_input_bytes = serialize signature_input sig_input in
-    guard (verify vk_sender sig_input_bytes msg_signed.signature);?
-    guard (msg_signed.receiver = receiver);?
-    Some ({sender=msg_signed.sender; receiver; payload=msg_signed.payload} <: communication_message)
-  ) else (
-    let sig_input = Plain {sender=msg_signed.sender; receiver=msg_signed.receiver; payload=msg_signed.payload} in
-    let sig_input_bytes = serialize signature_input sig_input in
-    guard (verify vk_sender sig_input_bytes msg_signed.signature);?
-    guard (msg_signed.receiver = receiver);?
-    Some ({sender=msg_signed.sender; receiver; payload=msg_signed.payload} <: communication_message)
+  let? sign_input = parse signature_input msg_signed.payload in
+  match sign_input with
+  | Plain cm -> (
+    guard (verify vk_sender msg_signed.payload msg_signed.signature);?
+    guard (cm.receiver = receiver);?
+    Some cm.payload
   )
+  | Encrypted payload -> (
+    guard (verify vk_sender msg_signed.payload msg_signed.signature);?
+    //guard (msg_signed.receiver = receiver);?
+    //guard (DY.Core.Bytes.Type.PkEnc? msg_signed.payload);?
+    Some payload
+  )
+#pop-options
 
-val get_sender: bytes -> option principal
-let get_sender msg_bytes =
+val parse_sig_message: bytes -> option communication_message
+let parse_sig_message msg_bytes =
   let? msg = parse communication_message_sign msg_bytes in
-  Some msg.sender
+  let? sign_input = parse signature_input msg.payload in
+  guard(Plain? sign_input);?
+  Some (Plain?.msg sign_input)
 
 val receive_authenticated:
   communication_keys_sess_ids ->
   principal -> timestamp ->
   traceful (option communication_message)
 let receive_authenticated comm_keys_ids receiver msg_id =
-  let*? msg_signed_bytes = recv_msg msg_id in
-  let*? sender = return (get_sender msg_signed_bytes) in
-  let*? vk_sender = get_public_key receiver comm_keys_ids.pki (LongTermSigKey comm_layer_sign_tag) sender in
-  let*? cm:communication_message = return (verify_message receiver msg_signed_bytes false vk_sender) in
-  trigger_event receiver (CommAuthReceiveMsg sender receiver cm.payload);*
-  return (Some cm)
-
+  let*? msg_signed = recv_msg msg_id in
+  let*? msg:communication_message = return (parse_sig_message msg_signed) in
+  let*? vk_sender = get_public_key receiver comm_keys_ids.pki (LongTermSigKey comm_layer_sign_tag) msg.sender in
+  let*? payload = return (verify_message receiver msg_signed false vk_sender) in
+  trigger_event receiver (CommAuthReceiveMsg msg.sender receiver msg.payload);*
+  return (Some msg)
 
 (**** Confidential and Authenticates Send and Receive Functions ****)
 
 val encrypt_and_sign_message: principal -> principal -> bytes -> bytes -> bytes -> bytes -> bytes -> bytes
 let encrypt_and_sign_message sender receiver payload pk_receiver sk_sender enc_nonce sign_nonce =
-  let enc_payload = encrypt_message pk_receiver enc_nonce payload in
+  let pkenc_sign_input = PkEncSignInput {sender; receiver; payload} in
+  let enc_payload = encrypt_message pk_receiver enc_nonce pkenc_sign_input in
   sign_message sender receiver enc_payload true sk_sender sign_nonce
 
+// TODO remove comment if proof works
 // We do not encrypt the sender and receiver
 // because, in real-world settings, they can also
 // be identified by the IP addresses or
@@ -219,23 +239,28 @@ let send_confidential_authenticated comm_keys_ids sender receiver payload =
   let* msg_id = send_msg msg_encrypted_signed_bytes in
   return (Some msg_id)
 
-val verify_and_decrypt_message: principal -> bytes -> bytes -> bytes -> option communication_message
-let verify_and_decrypt_message receiver msg_encrypted_signed sk_receiver vk_sender =
-  let? cm:communication_message = verify_message receiver msg_encrypted_signed true vk_sender in
-  let? payload = decrypt_message sk_receiver cm.payload in
-  Some ({cm with payload} <: communication_message)
+val decrypt_signed_message: principal -> bytes -> bytes -> option communication_message
+let decrypt_signed_message receiver sk_receiver msg_encrypted_signed =
+  let? signed_msg = parse communication_message_sign msg_encrypted_signed in
+  let? signature_in = parse signature_input signed_msg.payload in
+  guard(Encrypted? signature_in);?
+  let? pkenc_in = decrypt_message sk_receiver (Encrypted?.payload signature_in) in 
+  guard(PkEncSignInput? pkenc_in);?
+  let cm = PkEncSignInput?.cm pkenc_in in
+  guard(cm.receiver = receiver);?
+  Some cm
 
 val receive_confidential_authenticated:
   communication_keys_sess_ids ->
   principal -> timestamp ->
   traceful (option communication_message)
 let receive_confidential_authenticated comm_keys_ids receiver msg_id =
-  let*? msg_encrypted_signed_bytes = recv_msg msg_id in
-  let*? sender = return (get_sender msg_encrypted_signed_bytes) in
+  let*? msg_encrypted_signed = recv_msg msg_id in
   let*? sk_receiver = get_private_key receiver comm_keys_ids.private_keys (LongTermPkEncKey comm_layer_pkenc_tag) in
-  let*? vk_sender = get_public_key receiver comm_keys_ids.pki (LongTermSigKey comm_layer_sign_tag) sender in
-  let*? cm:communication_message = return (verify_and_decrypt_message receiver msg_encrypted_signed_bytes sk_receiver vk_sender) in  
-  trigger_event receiver (CommConfAuthReceiveMsg sender receiver cm.payload);*
+  let*? cm:communication_message = return (decrypt_signed_message receiver sk_receiver msg_encrypted_signed) in  
+  let*? vk_sender = get_public_key receiver comm_keys_ids.pki (LongTermSigKey comm_layer_sign_tag) cm.sender in
+  let*? _ = return (verify_message receiver msg_encrypted_signed true vk_sender) in  
+  trigger_event receiver (CommConfAuthReceiveMsg cm.sender receiver cm.payload);*
   return (Some cm)
 
 
